\newcommand\tab[1][1cm]{\hspace*{#1}}
\begin{answer}
  \\ \\
  \tab[2.25cm]$\frac{\partial}{\partial\eta}p(y;\eta) = p(y;n)(y-\frac{\partial}{\partial\eta}a(\eta)) $ \\ \\
  \tab[2.25cm]$\int\frac{\partial}{\partial\eta}p(y;\eta)dy = \int p(y;n)(y-\frac{\partial}{\partial\eta}a(\eta))dy $ \\ \\
  \tab[3.75cm]$=\int yp(y;\eta)dy - \int p(y;n) \frac{\partial}{\partial\eta}a(\eta)dy$ \\ \\
   \tab[2.25cm]$ \frac{\partial}{\partial\eta} = E[Y;\eta] - \frac{\partial}{\partial\eta}a(\eta)\int p(y;\eta)dy$ \\ \\
   \tab[2.25cm]$ E(y;\eta) = \frac{\partial}{\partial\eta}a(\eta)$ \\ \\
\end{answer}
